src/lemmas.lean
@@ -10,14 +10,6 @@ import defs
 namespace coc
 section
 
-/- Notations. -/
-
-set_option pp.beta true
-set_option pp.structure_projections false
-
-local notation e ` ⟦` n ` ↦ ` e' `⟧` := expr.subst e n e'
-local notation e ` ⟦` n ` ↟ ` m `⟧`  := expr.shift e n m
-
 /- Auxiliary arithmetic lemmas. -/
 
 lemma nat.order_aux_1 {a b : nat} (h₁ : ¬a < b) (h₂ : ¬a = b) : (b < a) := ne.lt_of_le (ne.symm h₂) (le_of_not_gt h₁)
@@ -34,8 +26,36 @@ lemma nat.le_add_right' (a b c : ℕ) (h : a ≤ b) : a ≤ b + c := by
   refine @nat.le.intro _ _ (k + c) _,
   rw [← nat.add_assoc, hk] }
 
+lemma list.nth_aux_1 {α} (a b : list α) (n : nat) (h : n < a.length) :
+  list.nth (a ++ b) n = list.nth a n := by
+{ exact list.nth_append h }
+
+lemma list.nth_aux_2 {α} (a b : list α) (n : nat) :
+  list.nth (a ++ b) (a.length + n) = list.nth b n := by
+{ rw [nat.add_comm, list.nth_append_right (nat.le_add_left _ _), nat.add_sub_cancel _ _] }
+
+lemma list.nth_aux_3 {α} (a : list α) (b : α) (c : list α) (n : nat) (h : n < a.length) :
+  list.nth (a ++ b :: c) n = list.nth a n := by
+{ exact list.nth_append h }
+
+lemma list.nth_aux_4 {α} (a : list α) (b : α) (c : list α) :
+  list.nth (a ++ b :: c) a.length = option.some b := by
+{ rw [← nat.zero_add a.length, list.nth_append_right (nat.le_add_left _ _), nat.add_sub_cancel _ _], refl }
+
+lemma list.nth_aux_5 {α} (a : list α) (b : α) (c : list α) (n : nat) :
+  list.nth (a ++ b :: c) (a.length + n.succ) = list.nth c n := by
+{ rw [nat.add_comm, list.nth_append_right (nat.le_add_left _ _), nat.add_sub_cancel _ _], refl }
+
 namespace expr
 section
+
+/- Notations. -/
+
+set_option pp.beta true
+set_option pp.structure_projections false
+
+local notation e ` ⟦` n ` ↦ ` e' `⟧` := subst e n e'
+local notation e ` ⟦` n ` ↟ ` m `⟧`  := shift e n m
 
 /- Uninteresting `shift` lemmas for supporting case analysis. -/
 
@@ -893,6 +913,7 @@ lemma has_type_unique {Γ e t} (h : Γ ▷ e : t) {t'} (h' : Γ ▷ e : t') : t 
 
 /-- Typing judgment lemmas. -/
 
+/-
 lemma has_type_conv {Γ e t' s} (t) (hc : t ~~ t') (hs : Γ ▷ t' : sort s) (h' : Γ ▷ e : t) :
   Γ ▷ e : t' := t_conv hc hs h'
 
@@ -937,19 +958,271 @@ lemma has_type_pi {Γ t₁ t₂ t} (h : Γ ▷ pi t₁ t₂ : t) :
     exact ⟨s₁, s₂, ih₁, ih₂, se_trans (se_symm hc) ih₃⟩ },
   case t_pi : _ _ s₁ _ s₂ ht₁ ht₂ _ _
   { exact ⟨s₁, s₂, ht₁, ht₂, se_refl⟩ } }
+-/
 
-lemma well_ctx_has_type_sort {Γ n t} (hw : ▷ Γ) (h : list.nth Γ n = option.some t) :
-  ∃ s, (Γ ▷ t ⟦0 ↟ n.succ⟧ : sort s) := by
+/- Auxiliary functions and related lemmas. -/
+
+def ctx_shift : ctx → nat → ctx
+| []       _ := []
+| (t :: Γ) n := (t ⟦Γ.length ↟ n⟧) :: ctx_shift Γ n
+
+def ctx_subst : ctx → expr → ctx
+| []       _ := []
+| (t :: Γ) e := (t ⟦Γ.length ↦ e⟧) :: ctx_subst Γ e
+
+local notation `|` Γ `|`       := list.length Γ
+local notation Γ ` ⟦↦↦ ` e `⟧` := ctx_subst Γ e
+local notation Γ ` ⟦↟↟ ` n `⟧` := ctx_shift Γ n
+
+lemma ctx_shift_length (Γ e) : |(Γ ⟦↟↟ e⟧)| = |Γ| := by
 { induction Γ with t Γ ih,
-  { injections },
-  { cases n with n,
-    { rcases hw with _ | @⟨_, _, s, hw, ht⟩,
-      unfold list.nth at h,
-      injection h with h,
-      rw ← h,
-      refine ⟨s, _⟩,
-      sorry },
-    { sorry } } }
+  { unfold ctx_shift },
+  { unfold ctx_shift list.length at *, rw ih } }
+
+lemma ctx_shift_nth {Γ n e} (h : list.nth Γ n = option.some e) {m} (h' : n.succ + m = |Γ|) (k) :
+  list.nth (Γ ⟦↟↟ k⟧) n = option.some (e ⟦m ↟ k⟧) := by
+{ induction Γ with t Γ ih generalizing n,
+  { unfold list.nth at h, injection h },
+  { unfold ctx_shift at ih ⊢,
+    cases n with n,
+    { unfold list.nth list.length at *, injection h with h,
+      rw [nat.one_add, nat.add_one] at h', injection h' with h',
+      rw [h, h'] },
+    { unfold list.nth list.length at *,
+      rw [nat.add_one, nat.succ_add] at h', injection h' with h',
+      exact ih h h' } } }
+
+lemma ctx_subst_length (Γ e) : |(Γ ⟦↦↦ e⟧)| = |Γ| := by
+{ induction Γ with t Γ ih,
+  { unfold ctx_subst },
+  { unfold ctx_subst list.length at *, rw ih } }
+
+lemma ctx_subst_nth {Γ n e} (h : list.nth Γ n = option.some e) {m} (h' : n.succ + m = |Γ|) (e') :
+  list.nth (Γ ⟦↦↦ e'⟧) n = option.some (e ⟦m ↦ e'⟧) := by
+{ induction Γ with t Γ ih generalizing n,
+  { unfold list.nth at h, injection h },
+  { unfold ctx_subst at ih ⊢,
+    cases n with n,
+    { unfold list.nth list.length at *, injection h with h,
+      rw [nat.one_add, nat.add_one] at h', injection h' with h',
+      rw [h, h'] },
+    { unfold list.nth list.length at *,
+      rw [nat.add_one, nat.succ_add] at h', injection h' with h',
+      exact ih h h' } } }
+
+/- How typing interacts with shifting. -/
+
+/-- Lean 3 does not have good specialised support mutually inductive types.
+    To carry out proofs using mutual induction, we have to define both statements beforehand. -/
+def judgment_shift_ind_type : judgment_index → Prop
+| (well_ctx Γ₀) :=
+  ∀ {Γ' Γ} (h₀ : Γ₀ = Γ' ++ Γ) (h : ▷ (Γ' ++ Γ)) {Δ} (hw : ▷ (Δ ++ Γ)),
+  ▷ (Γ' ⟦↟↟ |Δ|⟧) ++ Δ ++ Γ
+| (has_type Γ₀ e t) :=
+  ∀ {Γ' Γ} (h₀ : Γ₀ = Γ' ++ Γ) (h : (Γ' ++ Γ) ▷ e : t) {Δ} (hw : ▷ (Δ ++ Γ)),
+  (Γ' ⟦↟↟ |Δ|⟧ ++ Δ ++ Γ) ▷ e ⟦|Γ'| ↟ |Δ|⟧ : t ⟦|Γ'| ↟ |Δ|⟧
+
+/-- The mutual induction proof itself. -/
+lemma judgment_shift_ind (i : judgment_index) (h : judgment i) : judgment_shift_ind_type i := by
+{ induction h,
+  case c_nil
+  { unfold judgment_shift_ind_type at *, intros Γ' Γ h₀ h Δ hw, rw list.nil_eq_append_iff at h₀,
+    rw h₀.1 at h ⊢, rw h₀.2 at h hw ⊢,
+    exact hw },
+  case c_cons : Γ₀ t s hw ht ihw iht
+  { unfold judgment_shift_ind_type at *, intros Γ' Γ h₀ h Δ hw',
+    cases Γ' with t' Γ' ih',
+    { unfold ctx_shift, exact hw' },
+    { rw list.cons_append at h₀, injection h₀ with h₁ h₂,
+      rw ← h₁ at h h₀ ⊢, clear h₁ t',
+      rw h₂ at hw ht ihw iht, clear h₂ h₀ Γ₀,
+      specialize ihw rfl hw hw',
+      specialize iht rfl ht hw', unfold shift at iht,
+      unfold ctx_shift,
+      exact c_cons ihw iht } },
+  case t_conv : Γ₀ e t t' s hc ht he iht ihe
+  { unfold judgment_shift_ind_type at *, intros Γ' Γ h₀ h Δ hw, rw h₀ at *, clear h₀ Γ₀,
+    specialize iht rfl ht hw, unfold shift at iht,
+    specialize ihe rfl he hw,
+    exact t_conv (small_eq_shift_ind hc _ _) iht ihe },
+  case t_sort : Γ₀ n hc ih 
+  { unfold judgment_shift_ind_type at *, intros Γ' Γ h₀ h Δ hw, rw h₀ at *, clear h₀ Γ₀,
+    specialize ih rfl hc hw,
+    unfold shift, exact t_sort ih },
+  case t_var : Γ₀ n t hc ht ih
+  { unfold judgment_shift_ind_type at *, intros Γ' Γ h₀ h Δ hw, rw h₀ at *, clear h₀ Γ₀,
+    specialize ih rfl hc hw,
+    rcases (lt_or_le n Γ'.length) with h₁ | h₁,
+    { rw shift_gt h₁,
+      obtain ⟨m, hm⟩ := nat.le.dest (nat.succ_le_of_lt h₁),
+      have := shift_shift_disjoint t n.succ m Δ.length,
+      rw hm at this, rw ← this, clear this,
+      refine t_var ih _,
+      have h₂ := h₁, rw ← @ctx_shift_length Γ' Δ.length at h₂,
+      rw [list.append_assoc, list.nth_aux_1 _ _ _ h₂],
+      rw list.nth_aux_1 _ _ _ h₁ at ht,
+      exact ctx_shift_nth ht hm _ },
+    { rw shift_le h₁,
+      obtain ⟨m, hm⟩ := nat.le.dest h₁,
+      have := shift_shift_overlap t Γ'.length m.succ Δ.length,
+      rw [nat.add_succ, hm] at this, rw [this, nat.succ_add], clear this,
+      refine t_var ih _,
+      rw [← hm, list.nth_aux_2] at ht,
+      have h₂ := hm, rw ← @ctx_shift_length Γ' Δ.length at h₂,
+      rw [← h₂, list.append_assoc, nat.add_assoc, list.nth_aux_2, nat.add_comm, list.nth_aux_2],
+      exact ht } },
+  case t_app : Γ₀ l r t₁ t₂ hl hr ihl ihr
+  { unfold judgment_shift_ind_type at *, intros Γ' Γ h₀ h Δ hw, rw h₀ at *, clear h₀ Γ₀,
+    specialize ihl rfl hl hw,
+    specialize ihr rfl hr hw,
+    unfold shift at *,
+    have := shift_subst_below_ind t₂ r 0 Γ'.length Δ.length,
+    rw nat.add_zero at this, rw ← this,
+    exact t_app ihl ihr },
+  case t_lam : Γ₀ t₁ t₂ s e hs he iht ihe
+  { unfold judgment_shift_ind_type at *, intros Γ' Γ h₀ h Δ hw, rw h₀ at *, clear h₀ Γ₀,
+    specialize iht rfl hs hw,
+    rw ← list.cons_append at he ihe,
+    specialize ihe rfl he hw, unfold ctx_shift at ihe,
+    unfold shift at *,
+    exact t_lam iht ihe },
+  case t_pi : Γ₀ t₁ s₁ t₂ s₂ ht₁ ht₂ iht₁ iht₂
+  { unfold judgment_shift_ind_type at *, intros Γ' Γ h₀ h Δ hw, rw h₀ at *, clear h₀ Γ₀,
+    specialize iht₁ rfl ht₁ hw,
+    rw ← list.cons_append at ht₂ iht₂,
+    specialize iht₂ rfl ht₂ hw, unfold ctx_shift at iht₂,
+    unfold shift at *,
+    exact t_pi iht₁ iht₂ } }
+
+lemma well_ctx_shift_ind {Γ' Γ} (h : ▷ Γ' ++ Γ) {Δ} (hw : ▷ Δ ++ Γ) :
+  ▷ (Γ' ⟦↟↟ |Δ|⟧) ++ Δ ++ Γ :=
+    judgment_shift_ind (well_ctx (Γ' ++ Γ)) h rfl h hw
+
+lemma well_ctx_shift {Γ} (h : ▷ Γ) {Δ} (hw : ▷ Δ ++ Γ) : -- This one is useless.
+  ▷ Δ ++ Γ := by
+{ rw ← list.nil_append Γ at h,
+  have := well_ctx_shift_ind h hw,
+  unfold ctx_shift list.append at this,
+  rw list.nil_append at this,
+  exact this }
+
+lemma has_type_shift_ind {Γ' Γ e t} (h : (Γ' ++ Γ) ▷ e : t) {Δ} (hw : ▷ (Δ ++ Γ)) :
+  (Γ' ⟦↟↟ |Δ|⟧ ++ Δ ++ Γ) ▷ e ⟦|Γ'| ↟ |Δ|⟧ : t ⟦|Γ'| ↟ |Δ|⟧ :=
+    judgment_shift_ind (has_type (Γ' ++ Γ) e t) h rfl h hw
+
+lemma has_type_shift {Γ e t} (h : Γ ▷ e : t) {Δ} (hw : ▷ (Δ ++ Γ)) :
+  (Δ ++ Γ) ▷ e ⟦0 ↟ |Δ|⟧ : t ⟦0 ↟ |Δ|⟧ := by
+{ rw ← list.nil_append Γ at h,
+  have := has_type_shift_ind h hw,
+  unfold ctx_shift list.length at this,
+  rw list.nil_append at this,
+  exact this }
+
+/-- How typing interacts with substitution. -/
+lemma has_type_subst_ind {Γ Δ l r t₁ t₂} (hl : (Γ ++ t₁ :: Δ) ▷ l : t₂) (hr : Δ ▷ r : t₁) :
+  (ctx_subst Γ r ++ Δ) ▷ l ⟦Γ.length ↦ r⟧ : t₂ ⟦Γ.length ↦ r⟧ := by
+{ revert_all, intros Γ₀ Δ₀ l₀ r₀ t₁₀ t₂₀ hl₀ hr₀,
+  induction' hl₀,
+  case t_conv : e t t' s hc ht he iht ihe
+  { unfold subst at iht,
+    exact t_conv (small_eq_subst_ind hc se_refl _) (iht hr₀) (ihe hr₀) },
+  case t_sort : n h ih
+  { unfold subst, exact t_sort },
+  case t_var : n t h ht ih
+  { rcases (nat.lt_trichotomy Γ₀.length n) with h₁ | h₁ | h₁,
+    { cases n with n, { exfalso, exact nat.not_lt_zero _ h₁ },
+      rw [subst_lt h₁],
+      replace h₁ := nat.le_of_lt_succ h₁,
+      obtain ⟨m, hm⟩ := nat.le.dest h₁,
+      have := @shift_subst_inside t r₀ Γ₀.length m.succ,
+      rw [nat.add_succ, hm] at this,
+      rw [this, nat.pred_succ], clear this,
+      refine t_var _,
+      have hm' := hm, rw [← @ctx_subst_length Γ₀ r₀] at hm',
+      rw [← hm', list.nth_aux_2],
+      rw [← hm, ← nat.add_succ, list.nth_aux_2] at h,
+      exact h },
+    { have := @shift_subst_inside t r₀ n 0,
+      rw [nat.add_zero] at this,
+      rw [h₁, subst_eq, this], clear this,
+      rw [← h₁, list.nth_aux_4] at h, injection h with h, rw h at hr₀,
+      have := has_type_shift (ctx_subst Γ₀ r₀) hr₀,
+      rw [ctx_subst_length, h₁] at this, exact this },
+    { rw [subst_gt h₁],
+      rw [list.nth_aux_3 _ _ _ _ h₁] at h,
+      have h₂ := nat.succ_le_of_lt h₁,
+      obtain ⟨m, hm⟩ := nat.le.dest h₂,
+      rw [← hm, shift_subst_above],
+      refine t_var _,
+      rw [← @ctx_subst_length Γ₀ r₀] at h₁,
+      rw [list.nth_aux_1 _ _ _ h₁],
+      exact ctx_subst_nth h hm } },
+  case t_app : l r t₁ t₂ hl hr ihl ihr
+  { unfold subst at ihl ⊢, rw ← subst_subst,
+    exact t_app (ihl hr₀) (ihr hr₀) },
+  case t_lam : t₁ t₂ s e hs he iht ihe
+  { unfold subst at iht ⊢,
+    refine t_lam (iht hr₀) _,
+    replace ihe := ihe hr₀ (list.cons_append _ _ _).symm,
+    unfold ctx_subst list.length at ihe,
+    rw [nat.add_one, list.cons_append] at ihe,
+    exact ihe },
+  case t_pi : t₁ s₁ t₂ s₂ ht₁ ht₂ iht₁ iht₂
+  { unfold subst at iht₁ ⊢,
+    refine t_pi (iht₁ hr₀) _,
+    replace iht₂ := iht₂ hr₀ (list.cons_append _ _ _).symm,
+    unfold ctx_subst list.length subst at iht₂,
+    rw [nat.add_one, list.cons_append] at iht₂,
+    exact iht₂ } }
+
+lemma has_type_subst {Γ l r t₁ t₂} (hl : (t₁ :: Γ) ▷ l : t₂) (hr : Γ ▷ r : t₁) :
+  Γ ▷ l ⟦0 ↦ r⟧ : t₂ ⟦0 ↦ r⟧ := by
+{ rw ← list.nil_append (t₁ :: Γ) at hl,
+  have := has_type_subst_ind hl hr,
+  unfold ctx_subst at this,
+  rw list.nil_append at this,
+  exact this }
+
+lemma has_type_cons {Γ e t} (h : Γ ▷ e : t) {t' s} (hw : Γ ▷ t' : sort s) :
+  (t' :: Γ) ▷ e ⟦0 ↟ 1⟧ : t ⟦0 ↟ 1⟧ := by
+{ induction' h,
+  case t_conv : Γ e t t'' s hc ht he iht ihe
+  { specialize iht hw, unfold shift at iht,
+    exact t_conv (small_eq_shift hc 1) iht (ihe hw) },
+  case t_sort : Γ n h ih
+  { clear ih, unfold shift, exact t_sort (c_cons h hw) },
+  case t_var : Γ n t h ht ih
+  { clear ih, rw shift_le (nat.zero_le _),
+    have h₁ := shift_shift_overlap t 0 n.succ 1, rw nat.zero_add at h₁, rw h₁,
+    exact t_var (c_cons h hw) ht },
+  case t_app : Γ l r t₁ t₂ hl hr ihl ihr
+  { unfold shift at ihl ⊢,
+    have h₁ := shift_subst_below t₂ r 0 1, rw ← h₁,
+    exact t_app (ihl hw) (ihr hw) },
+  case t_lam : Γ t₁ t₂ s e hs he iht ihe
+  { unfold shift at iht ⊢,
+    refine t_lam (iht hw) _, },
+  case t_pi : Γ t₁ s₁ t₂ s₂ ht₁ ht₂ iht₁ iht₂ { sorry } }
+
+lemma has_type_of_well_ctx_nth {Γ} (hw : ▷ Γ) {n t} (h : list.nth Γ n = option.some t) :
+  ∃ s, (Γ ▷ t ⟦0 ↟ n.succ⟧ : sort s) := by
+{ revert_after hw,
+  induction' hw,
+  case c_nil { intros, injections },
+  case c_cons : Γ t s hw ht ihw iht
+  { intros n t',
+    clear iht,
+    cases n with n,
+    { intros h, injection h with h,
+      have h₁ := has_type_cons ht ht, unfold shift at h₁,
+      rw h at h₁ ⊢,
+      exact ⟨s, h₁⟩ },
+    { intros h, unfold list.nth at h,
+      obtain ⟨s, hs⟩ := ihw h,
+      have h₁ := has_type_cons hs ht, unfold shift at h₁,
+      have h₂ := shift_shift_overlap t' 0 n.succ 1, rw nat.zero_add at h₂,
+      rw h₂ at h₁,
+      exact ⟨s, h₁⟩ } } }
 
 /-- Definitional equality for contexts. -/
 inductive small_eq_ctx : ctx → ctx → Prop
@@ -986,6 +1259,8 @@ lemma small_eq_ctx_elem {Γ Γ' n t} (he : Γ ~~c Γ') (h : Γ.nth n = option.so
     { unfold list.nth at h ⊢,
       exact ih h } } }
 
+-- I NEED SOMETHING LIKE "well_ctx_of_has_type"...
+
 /-- A term has equal types under equal contexts. -/
 lemma has_type_small_eq_ctx {Γ e t} (h : Γ ▷ e : t) {Γ'} (hw : ▷ Γ') (he : Γ ~~c Γ') : Γ' ▷ e : t := by
 { revert_all, intros Γ₀ e₀ t₀ h₀ Γ₀' hw₀ he₀, revert_after h₀,
@@ -1001,191 +1276,6 @@ lemma has_type_small_eq_ctx {Γ e t} (h : Γ ▷ e : t) {Γ'} (hw : ▷ Γ') (he
   case t_app : Γ l r t₁ t₂ hl hr ihl ihr { exact t_app (ihl he₀) (ihr he₀) },
   case t_lam : Γ t₁ t₂ s e hs he iht ihe { exact t_lam (iht he₀) (ihe (sec_cons se_refl he₀)) },
   case t_pi : Γ t₁ s₁ t₂ s₂ ht₁ ht₂ iht₁ iht₂ { exact t_pi (iht₁ he₀) (iht₂ (sec_cons se_refl he₀)) } }
-
-/- Main part. (Ugly!) -/
-
-/- Auxiliary functions and related lemmas. -/
-
-def ctxshift : ctx → nat → ctx
-| []       _ := []
-| (t :: Γ) n := (t ⟦Γ.length ↟ n⟧) :: ctxshift Γ n
-
-lemma ctxshift_length {Γ e} : (ctxshift Γ e).length = Γ.length := by
-{ induction Γ with t Γ ih,
-  { unfold ctxshift },
-  { unfold ctxshift list.length at *, rw ih } }
-
-lemma ctxshift_nth {Γ : ctx} {n m : nat} {e k} (h : Γ.nth n = option.some e) (h' : n.succ + m = Γ.length) :
-  (ctxshift Γ k).nth n = option.some (e ⟦m ↟ k⟧) := by
-{ induction' Γ with t Γ ih,
-  { unfold list.nth at h, injection h },
-  { unfold ctxshift at *,
-    cases n with n,
-    { unfold list.nth list.length at *, injection h with h,
-      rw [nat.one_add, nat.add_one] at h', injection h' with h',
-      rw [h, h'] },
-    { unfold list.nth list.length at *,
-      rw [nat.add_one, nat.succ_add] at h', injection h' with h',
-      exact ih h h' } } }
-
-def ctxsubst : ctx → expr → ctx
-| []       _ := []
-| (t :: Γ) e := (t ⟦Γ.length ↦ e⟧) :: ctxsubst Γ e
-
-lemma ctxsubst_length {Γ e} : (ctxsubst Γ e).length = Γ.length := by
-{ induction Γ with t Γ ih,
-  { unfold ctxsubst },
-  { unfold ctxsubst list.length at *, rw ih } }
-
-lemma ctxsubst_nth {Γ : ctx} {n m : nat} {e e'} (h : Γ.nth n = option.some e) (h' : n.succ + m = Γ.length) :
-  (ctxsubst Γ e').nth n = option.some (e ⟦m ↦ e'⟧) := by
-{ induction' Γ with t Γ ih,
-  { unfold list.nth at h, injection h },
-  { unfold ctxsubst at *,
-    cases n with n,
-    { unfold list.nth list.length at *, injection h with h,
-      rw [nat.one_add, nat.add_one] at h', injection h' with h',
-      rw [h, h'] },
-    { unfold list.nth list.length at *,
-      rw [nat.add_one, nat.succ_add] at h', injection h' with h',
-      exact ih h h' } } }
-
-lemma list.nth_aux_1 {α} (a b : list α) (n : nat) (h : n < a.length) :
-  list.nth (a ++ b) n = list.nth a n := by
-{ exact list.nth_append h }
-
-lemma list.nth_aux_2 {α} (a b : list α) (n : nat) :
-  list.nth (a ++ b) (a.length + n) = list.nth b n := by
-{ rw [nat.add_comm, list.nth_append_right (nat.le_add_left _ _), nat.add_sub_cancel _ _] }
-
-lemma list.nth_aux_3 {α} (a : list α) (b : α) (c : list α) (n : nat) (h : n < a.length) :
-  list.nth (a ++ b :: c) n = list.nth a n := by
-{ exact list.nth_append h }
-
-lemma list.nth_aux_4 {α} (a : list α) (b : α) (c : list α) :
-  list.nth (a ++ b :: c) a.length = option.some b := by
-{ rw [← nat.zero_add a.length, list.nth_append_right (nat.le_add_left _ _), nat.add_sub_cancel _ _], refl }
-
-lemma list.nth_aux_5 {α} (a : list α) (b : α) (c : list α) (n : nat) :
-  list.nth (a ++ b :: c) (a.length + n.succ) = list.nth c n := by
-{ rw [nat.add_comm, list.nth_append_right (nat.le_add_left _ _), nat.add_sub_cancel _ _], refl }
-
-/-- How typing interacts with shifting. -/
-lemma has_type_shift_ind (Δ : ctx) {Γ' Γ e t} (h : Γ' ++ Γ ▷ e : t) :
-  ctxshift Γ' Δ.length ++ Δ ++ Γ ▷ e ⟦Γ'.length ↟ Δ.length⟧ : t ⟦Γ'.length ↟ Δ.length⟧ := by
-{ induction' h,
-  case t_conv : e t t' s hc ht he iht ihe
-  { unfold shift at iht, exact t_conv (small_eq_shift_ind hc _ _) (iht _) (ihe _) },
-  case t_sort : n h ih
-  { unfold shift, exact t_sort },
-  case t_var : n t h ht ih
-  { rcases (lt_or_le n Γ'.length) with h₁ | h₁,
-    { rw shift_gt h₁,
-      obtain ⟨m, hm⟩ := nat.le.dest (nat.succ_le_of_lt h₁),
-      have := shift_shift_disjoint t n.succ m Δ.length,
-      rw hm at this, rw ← this, clear this,
-      refine t_var _,
-      have h₂ := h₁, rw ← @ctxshift_length Γ' Δ.length at h₂,
-      rw [list.append_assoc, list.nth_aux_1 _ _ _ h₂],
-      rw list.nth_aux_1 _ _ _ h₁ at h,
-      exact ctxshift_nth h hm },
-    { rw shift_le h₁,
-      obtain ⟨m, hm⟩ := nat.le.dest h₁,
-      have := shift_shift_overlap t Γ'.length m.succ Δ.length,
-      rw [nat.add_succ, hm] at this, rw [this, nat.succ_add], clear this,
-      refine t_var _,
-      rw [← hm, list.nth_aux_2] at h,
-      have h₂ := hm, rw ← @ctxshift_length Γ' Δ.length at h₂,
-      rw [← h₂, list.append_assoc, nat.add_assoc, list.nth_aux_2, nat.add_comm, list.nth_aux_2],
-      exact h } },
-  case t_app : l r t₁ t₂ hl hr ihl ihr
-  { unfold shift at *,
-    have := shift_subst_below_ind t₂ r 0 Γ'.length Δ.length,
-    rw nat.add_zero at this, rw ← this,
-    exact t_app (ihl _) (ihr _) },
-  case t_lam : t₁ t₂ s e hs he iht ihe
-  { unfold shift at *,
-    refine t_lam (iht _) _,
-    refine @ihe Δ (t₁ :: Γ') Γ e t₂ _,
-    rw list.cons_append _ _ _ },
-  case t_pi : t₁ s₁ t₂ s₂ ht₁ ht₂ iht₁ iht₂
-  { unfold shift at *,
-    refine t_pi (iht₁ _) _,
-    have := @iht₂ Δ (t₁ :: Γ') Γ t₁ t₂ _,
-    rw list.cons_append _ _ _, } }
-
-lemma has_type_shift (Δ : ctx) {Γ e t} (h : Γ ▷ e : t) :
-  Δ ++ Γ ▷ e ⟦0 ↟ Δ.length⟧ : t ⟦0 ↟ Δ.length⟧ := by
-{ rw ← list.nil_append Γ at h,
-  have := has_type_shift_ind Δ h,
-  unfold ctxshift list.length at this,
-  rw list.nil_append at this,
-  exact this }
-
-/-- How typing interacts with substitution. -/
-lemma has_type_subst_ind {Γ Δ l r t₁ t₂} (hl : Γ ++ t₁ :: Δ ▷ l : t₂) (hr : Δ ▷ r : t₁) :
-  ctxsubst Γ r ++ Δ ▷ l ⟦Γ.length ↦ r⟧ : t₂ ⟦Γ.length ↦ r⟧ := by
-{ revert_all, intros Γ₀ Δ₀ l₀ r₀ t₁₀ t₂₀ hl₀ hr₀,
-  induction' hl₀,
-  case t_conv : e t t' s hc ht he iht ihe
-  { unfold subst at iht,
-    exact t_conv (small_eq_subst_ind hc se_refl _) (iht hr₀) (ihe hr₀) },
-  case t_sort : n h ih
-  { unfold subst, exact t_sort },
-  case t_var : n t h ht ih
-  { rcases (nat.lt_trichotomy Γ₀.length n) with h₁ | h₁ | h₁,
-    { cases n with n, { exfalso, exact nat.not_lt_zero _ h₁ },
-      rw [subst_lt h₁],
-      replace h₁ := nat.le_of_lt_succ h₁,
-      obtain ⟨m, hm⟩ := nat.le.dest h₁,
-      have := @shift_subst_inside t r₀ Γ₀.length m.succ,
-      rw [nat.add_succ, hm] at this,
-      rw [this, nat.pred_succ], clear this,
-      refine t_var _,
-      have hm' := hm, rw [← @ctxsubst_length Γ₀ r₀] at hm',
-      rw [← hm', list.nth_aux_2],
-      rw [← hm, ← nat.add_succ, list.nth_aux_2] at h,
-      exact h },
-    { have := @shift_subst_inside t r₀ n 0,
-      rw [nat.add_zero] at this,
-      rw [h₁, subst_eq, this], clear this,
-      rw [← h₁, list.nth_aux_4] at h, injection h with h, rw h at hr₀,
-      have := has_type_shift (ctxsubst Γ₀ r₀) hr₀,
-      rw [ctxsubst_length, h₁] at this, exact this },
-    { rw [subst_gt h₁],
-      rw [list.nth_aux_3 _ _ _ _ h₁] at h,
-      have h₂ := nat.succ_le_of_lt h₁,
-      obtain ⟨m, hm⟩ := nat.le.dest h₂,
-      rw [← hm, shift_subst_above],
-      refine t_var _,
-      rw [← @ctxsubst_length Γ₀ r₀] at h₁,
-      rw [list.nth_aux_1 _ _ _ h₁],
-      exact ctxsubst_nth h hm } },
-  case t_app : l r t₁ t₂ hl hr ihl ihr
-  { unfold subst at ihl ⊢, rw ← subst_subst,
-    exact t_app (ihl hr₀) (ihr hr₀) },
-  case t_lam : t₁ t₂ s e hs he iht ihe
-  { unfold subst at iht ⊢,
-    refine t_lam (iht hr₀) _,
-    replace ihe := ihe hr₀ (list.cons_append _ _ _).symm,
-    unfold ctxsubst list.length at ihe,
-    rw [nat.add_one, list.cons_append] at ihe,
-    exact ihe },
-  case t_pi : t₁ s₁ t₂ s₂ ht₁ ht₂ iht₁ iht₂
-  { unfold subst at iht₁ ⊢,
-    refine t_pi (iht₁ hr₀) _,
-    replace iht₂ := iht₂ hr₀ (list.cons_append _ _ _).symm,
-    unfold ctxsubst list.length subst at iht₂,
-    rw [nat.add_one, list.cons_append] at iht₂,
-    exact iht₂ } }
-
-lemma has_type_subst {Γ l r t₁ t₂} (hl : t₁ :: Γ ▷ l : t₂) (hr : Γ ▷ r : t₁) :
-  Γ ▷ l ⟦0 ↦ r⟧ : t₂ ⟦0 ↦ r⟧ := by
-{ rw ← list.nil_append (t₁ :: Γ) at hl,
-  have := has_type_subst_ind hl hr,
-  unfold ctxsubst at this,
-  rw list.nil_append at this,
-  exact this }
 
 /-- Small-step reduction preserves type. -/
 lemma has_type_small {Γ e e' t} (h : Γ ▷ e : t) (h' : e ~> e') : (Γ ▷ e' : t) := by
