src/tactics.lean
@@ -1,0 +1,72 @@
+import init.meta.tactic
+import tactic.interactive
+
+namespace tactic.interactive
+
+open tactic
+open interactive
+
+/-- Unmodified core implementation. -/
+private meta def goals_with_matching_tag (ns : list name) : tactic (list (expr × case_tag) × list (expr × case_tag)) := do
+  gs ← get_goals,
+  (gs : list (expr × tag)) ← gs.mmap (λ g, do t ← get_tag g, pure (g, t)),
+  pure $ gs.foldr
+    (λ ⟨g, t⟩ ⟨exact_matches, suffix_matches⟩,
+      match case_tag.parse t with
+      | none := ⟨exact_matches, suffix_matches⟩
+      | some t :=
+        match case_tag.match_tag ns t with
+        | case_tag.match_result.exact_match := ⟨⟨g, t⟩ :: exact_matches, suffix_matches⟩
+        | case_tag.match_result.fuzzy_match := ⟨exact_matches, ⟨g, t⟩ :: suffix_matches⟩
+        | case_tag.match_result.no_match    := ⟨exact_matches, suffix_matches⟩
+        end
+      end)
+    ([], [])
+
+/-- Modified core implementation to allow multiple goals with the given suffix
+    (in which case it chooses the first one). -/
+private meta def goal_with_matching_tag (ns : list name) : tactic (expr × case_tag) := do
+  ⟨exact_matches, suffix_matches⟩ ← goals_with_matching_tag ns,
+  match exact_matches, suffix_matches with
+  | [],        []        := fail format! "Invalid `case`: there is no goal tagged with suffix {ns}."
+  | [],        (g :: gs) := pure g
+  | (g :: gs), _         := pure g
+  end
+
+/-- Unmodified core implementation. -/
+meta def case' (args : parse case_parser) (tac : itactic) : tactic unit := do
+  target_goals ← args.mmap (λ ⟨ns, ids⟩, do
+    ⟨goal, tag⟩ ← goal_with_matching_tag ns,
+    let ids := ids.get_or_else [],
+    let num_ids := ids.length,
+    goals ← get_goals,
+    let other_goals := goals.filter (≠ goal),
+    set_goals [goal],
+    match tag with
+    | (case_tag.pi _ num_args) := do
+      intro_lst ids,
+      when (num_ids < num_args) $ intron (num_args - num_ids)
+    | (case_tag.hyps _ new_hyp_names) := do
+        let num_new_hyps := new_hyp_names.length,
+        when (num_ids > num_new_hyps) $ fail format!
+          ("Invalid `case`: You gave {num_ids} names, but the case introduces " ++
+          "{num_new_hyps} new hypotheses."),
+        let renamings := native.rb_map.of_list (new_hyp_names.zip ids),
+        propagate_tags $ tactic.rename_many renamings tt tt
+    end,
+    goals ← get_goals,
+    set_goals other_goals,
+    match goals with
+    | [g] := return g
+    | _ := fail "Unexpected goals introduced by renaming"
+    end),
+  remaining_goals ← get_goals,
+  set_goals target_goals,
+  tac,
+  unsolved_goals ← get_goals,
+  match unsolved_goals with
+  | [] := set_goals remaining_goals
+  | _  := fail "`case` tactic failed, focused goals have not been solved"
+  end
+
+end tactic.interactive
